extensionality of state dictionaries

lib/everparse/3d/EverParse3d.State.fst
@@ -2,12 +2,167 @@ module EverParse3d.State
 open Pulse.Lib.Pervasives
 open Pulse.Lib.ForEvery
 
+open FStar.FunctionalExtensionality
+
+let extensionality' (a: Type) (b: (a -> Type)) (f g: restricted_t a b)
+    : Lemma (requires feq #a #b f g) (ensures f == g)
+= ()
+
+let extensionality_g' (a: Type) (b: (a -> Type)) (f g: restricted_g_t a b)
+    : Lemma (requires feq_g #a #b f g) (ensures f == g)
+= ()
+
+module ID = FStar.IndefiniteDescription
+
+let arrow_g (t1: Type) (t2: Type) = t1 ^->> t2
+
+let refine_t (t: Type) (p: t `arrow_g` bool) = (x: t { p x })
+
+let restricted_t' (a: Type) (b: a -> Type) = restricted_t a (on_dom a b)
+
+let restricted_t'_eq (a1: Type) (b1: a1 -> Type) (a2: Type) (b2: a2 -> Type) : Lemma
+  (requires
+    a1 == a2 /\
+    feq b1 b2
+  )
+  (ensures restricted_t' a1 b1 == restricted_t' a2 b2)
+= ()
+
+let arrow (t1: Type) (t2: Type) = t1 ^-> t2
+
 inline_for_extraction noextract
 noeq type state_dict = {
-  state_p: string -> prop;
-  state_values: (x: string { state_p x }) -> Type0;
-  state: (x: string { state_p x }) -> state_values x -> slprop;
+  state_p: string `arrow_g` bool;
+  state_values: refine_t string state_p `arrow` Type0;
+  state: restricted_t' (refine_t string state_p) (fun x -> (state_values x `arrow` slprop));
 }
+
+let state_dict_ext
+  (d1 d2: state_dict)
+: Lemma
+  (requires (
+    (forall x . d1.state_p x == d2.state_p x) /\
+    (forall (x: refine_t string d1.state_p) . d1.state_values x == d2.state_values x) /\
+    (forall (x: refine_t string d1.state_p) (v: d1.state_values x) . d1.state x v == d2.state x v
+  )))
+  (ensures (
+    d1 == d2
+  ))
+= assert (feq_g (d1.state_p <: (string ^->> bool)) (d2.state_p <: (string ^->> bool)));
+  extensionality_g' string (fun _ -> bool) d1.state_p d2.state_p;
+  assert (d1.state_p == d2.state_p);
+  assert (refine_t string d1.state_p == refine_t string d2.state_p);
+  assert (refine_t string d1.state_p `arrow` Type0 == refine_t string d2.state_p `arrow` Type0);
+  assert (feq d1.state_values d2.state_values);
+  extensionality' (refine_t string d1.state_p) (fun _ -> Type0) d1.state_values (coerce_eq () d2.state_values <: refine_t string d1.state_p `arrow` Type0);
+  assert (d1.state_values == d2.state_values);
+  assert (forall (x: refine_t string d1.state_p) . feq (d1.state x) (d2.state x));
+  let prf
+    (x: refine_t string d1.state_p)
+  : Lemma (ensures d1.state x == d2.state x)
+    [SMTPat (d1.state x)]
+  =
+    assert (d1.state_values x `arrow` slprop == d2.state_values x `arrow` slprop);
+    extensionality' (d1.state_values x) (fun _ -> slprop) (d1.state x) (coerce_eq () (d2.state x) <: d1.state_values x `arrow` slprop)
+  in
+  assert (forall (x: refine_t string d1.state_p) . d1.state x == d2.state x);
+  restricted_t'_eq
+    (refine_t string d1.state_p) (fun x -> (d1.state_values x `arrow` slprop))
+    (refine_t string d2.state_p) (fun x -> (d2.state_values x `arrow` slprop));
+  assert (feq d1.state (coerce_eq () d2.state <: restricted_t' (refine_t string d1.state_p) (fun x -> (d1.state_values x `arrow` slprop))));
+  extensionality' (refine_t string d1.state_p) (on_dom (refine_t string d1.state_p) (fun x -> d1.state_values x ^-> slprop)) d1.state (coerce_eq () d2.state <: restricted_t' (refine_t string d1.state_p) (fun x -> (d1.state_values x `arrow` slprop)));
+  assert (d1.state == d2.state);
+  assert (d1 == d2)
+
+let mk_state_dict
+  (p: string -> prop)
+  (values: (x: string { p x }) -> Type0)
+  (state: (x: string { p x }) -> values x -> slprop)
+: Tot state_dict
+=
+  let p' = on_g string (fun x -> ID.strong_excluded_middle (p x) <: bool) in
+  let values' = on (refine_t string p') values in
+  let state' (x: refine_t string p') : (values' x ^-> slprop) = on (values' x) (state x) in
+  {
+    state_p = p';
+    state_values = values';
+    state = on_dom (refine_t string p') state';
+  }
+
+let mk_state_dict_correct
+  (p: string -> prop)
+  (values: (x: string { p x }) -> Type0)
+  (state: (x: string { p x }) -> values x -> slprop)
+: Lemma
+  (let d = mk_state_dict p values state in
+    (forall x . d.state_p x == true <==> p x) /\
+    (forall (x: string { p x }) . values x == d.state_values x) /\
+    (forall (x: refine_t string d.state_p) . d.state_values x == values x) /\
+    (forall (x: refine_t string d.state_p) (y: d.state_values x) . d.state x y == state x y) /\
+    (forall (x: string { p x }) (y: values x) . state x y == d.state x y)
+  )
+= let d = mk_state_dict p values state in
+  let prf
+    (x: refine_t string d.state_p)
+    (y: d.state_values x)
+  : Lemma
+    (d.state x y == state x y)
+  =
+    let p' = on_g string (fun x -> ID.strong_excluded_middle (p x) <: bool) in
+    assert (d.state_p == p');
+    let values' : refine_t string d.state_p `arrow` Type0 = on (refine_t string d.state_p) values in
+    assert_norm (d.state_values == (coerce_eq () values' <: (refine_t string d.state_p `arrow` Type0)));
+    let state' (x: refine_t string p') : (d.state_values x ^-> slprop) = on (d.state_values x) (state x) in
+    assert_norm (d.state == on_dom (refine_t string d.state_p) state');
+    assert_norm (d.state x == on_dom (refine_t string d.state_p) state' x);
+    assert (d.state x == state' x);
+    assert (d.state x y == state' x y);
+    assert (d.state x y == state x y)
+  in
+  Classical.forall_intro_2 prf
+
+let mk_state_dict_ext
+  (p1: string -> prop)
+  (values1: (x: string { p1 x }) -> Type0)
+  (state1: (x: string { p1 x }) -> values1 x -> slprop)
+  (p2: string -> prop)
+  (values2: (x: string { p2 x }) -> Type0)
+  (state2: (x: string { p2 x }) -> values2 x -> slprop)
+: Lemma
+  (requires (
+    (forall x . p1 x <==> p2 x) /\
+    (forall (x: string { p1 x }) . values1 x == values2 x) /\
+    (forall (x: string { p1 x }) (v: values1 x) . state1 x v == state2 x v)
+  ))
+  (ensures (mk_state_dict p1 values1 state1 == mk_state_dict p2 values2 state2))
+= let d1 = mk_state_dict p1 values1 state1 in
+  let d2 = mk_state_dict p2 values2 state2 in
+  assert (feq_g d1.state_p d2.state_p);
+  assert (feq d1.state_values d2.state_values);
+  restricted_t'_eq
+    (refine_t string d1.state_p) (fun x -> (d1.state_values x `arrow` slprop))
+    (refine_t string d2.state_p) (fun x -> (d2.state_values x `arrow` slprop));
+  let prf2
+    (x: refine_t string d1.state_p)
+  : Lemma
+    (d1.state x == (coerce_eq () (d2.state x) <: d1.state_values x `arrow` slprop))
+  =
+    mk_state_dict_correct p1 values1 state1;
+    mk_state_dict_correct p2 values2 state2;
+    assert (forall y . d1.state x y == d2.state x y);
+    assert (feq (d1.state x) (coerce_eq () (d2.state x) <: d1.state_values x `arrow` slprop));
+    extensionality' (d1.state_values x) (fun _ -> slprop) (d1.state x) (coerce_eq () (d2.state x) <: d1.state_values x `arrow` slprop)
+  in
+  Classical.forall_intro prf2;
+  assert (forall (x: refine_t string d1.state_p) . d1.state x == d2.state x);
+  assert (feq d1.state (coerce_eq () d2.state <: restricted_t' (refine_t string d1.state_p) (fun x -> (d1.state_values x `arrow` slprop))));
+  state_dict_ext d1 d2
+
+let state_p
+  (d: state_dict)
+  (x: string)
+: Tot prop
+= d.state_p x == true
 
 let forevery_values
       (p1: string -> prop)
@@ -17,23 +172,23 @@ let forevery_values
 
 let forevery_state
       (d: state_dict)
-      (v: forevery_values d.state_p d.state_values)
+      (v: forevery_values (state_p d) d.state_values)
 : Tot slprop
-= forall+ (x: string { d.state_p x }) . d.state x (v x)
+= forall+ (x: string { state_p d x }) . d.state x (v x)
 
 let state_dict_empty
-: state_dict = {
-  state_p = (fun _ -> False);
-  state_values = (fun _ -> unit);
-  state = (fun _ _ -> emp);
-}
+: state_dict =
+  mk_state_dict
+    (fun _ -> False)
+    (fun _ -> unit)
+    (fun _ _ -> emp)
 
 let state_dict_weaken_prop
   (d1 d2: state_dict)
 : Tot prop
-= (forall (x: string) . d1.state_p x ==> d2.state_p x) /\
-  (forall (x: string { d1.state_p x }) . d1.state_values x == d2.state_values x) /\
-  (forall (x: string { d1.state_p x }) . d1.state x == d2.state x)
+= (forall (x: string) . state_p d1 x ==> state_p d2 x) /\
+  (forall (x: string { state_p d1 x }) . d1.state_values x == d2.state_values x) /\
+  (forall (x: string { state_p d1 x }) . d1.state x == d2.state x)
 
 let forevery_singleton_prop
   (name: string)
@@ -61,8 +216,8 @@ let state_dict_singleton
   (name: string)
   (#t: Type0)
   (state: t -> slprop)
-: state_dict = {
-  state_p = forevery_singleton_prop name;
-  state_values = forevery_singleton_values name t;
-  state = forevery_singleton_state name state;
-}
+: state_dict =
+  mk_state_dict
+    (forevery_singleton_prop name)
+    (forevery_singleton_values name t)
+    (forevery_singleton_state name state)
